

$X \sim N(\mu, \sigma^2)$. $I(\mu, \sigma^2) = ((I_{ij}(\mu, \sigma^2)))$, where

$$I_{11}(\mu, \sigma^2) = E_{\mu, \sigma^2} \left[\frac{\partial}{\partial \mu} \log f(X|\mu, \sigma^2) \right]^2$$

$$I_{22}(\mu, \sigma^2) = E_{\mu, \sigma^2} \left[\frac{\partial}{\partial \sigma^2} \log f(X|\mu, \sigma^2) \right]^2$$

$$I_{12}(\mu, \sigma^2) = E_{\mu, \sigma^2} \left[\frac{\partial}{\partial \mu} \log f(X|\mu, \sigma^2) \frac{\partial}{\partial \sigma^2} \log f(X|\mu, \sigma^2) \right].$$

$$\log f(x|\mu, \sigma^2) = -\frac{1}{2} \log \sigma^2 - \frac{1}{2\sigma^2} (x - \mu)^2,$$

$$\frac{\partial}{\partial \mu} \log f(x|\mu, \sigma^2) = -\frac{1}{2\sigma^2} 2(x - \mu)(-1),$$

$$\frac{\partial}{\partial \sigma^2} \log f(x|\mu, \sigma^2) = -\frac{1}{2} \frac{1}{\sigma^2} + \frac{1}{2\sigma^4} (x - \mu)^2.$$

$$I_{11}(\mu, \sigma^2) = E_{\mu, \sigma^2} \left[\frac{(X - \mu)^2}{\sigma^4} \right] = \frac{1}{\sigma^2},$$

$$I_{22}(\mu, \sigma^2) = \frac{1}{4\sigma^8} E_{\mu, \sigma^2} [(X - \mu)^2 - \sigma^2]^2 = \frac{2\sigma^4}{4\sigma^8} = \frac{1}{2\sigma^4}.$$

$$I_{12}(\mu, \sigma^2) = \frac{1}{2} E_{\mu, \sigma^2} \left[\left(\frac{X - \mu}{\sigma^2} \right) \left(\frac{(X - \mu)^2 - \sigma^2}{\sigma^4} \right) \right] = 0.$$

$$I(\mu, \sigma^2) = \begin{pmatrix} \frac{1}{\sigma^2} & 0 \\ 0 & \frac{1}{2\sigma^4} \end{pmatrix}.$$

$$|I(\mu, \sigma^2)| \propto (\sigma^2)^{-3}.$$

Jeffreys (formal) prior is

$$\pi(\mu, \sigma^2) d\mu d\sigma^2 = |I(\mu, \sigma^2)|^{1/2} d\mu d\sigma^2 \propto (\sigma^2)^{-3/2} d\mu d\sigma^2.$$

Why is this not the same as the left invariant Haar measure on the affine group, which is

$$\sigma^{-2}?$$

Since $d\sigma^2 = 2\sigma d\sigma$,

$$\pi(\mu, \sigma) d\mu d\sigma \propto (\sigma^2)^{-3/2} d\mu \sigma d\sigma = \sigma^{-2} d\mu d\sigma.$$

$$\frac{P^\pi(\Theta_0|x)}{P^\pi(\Theta_1|x)} = \frac{P^\pi(\Theta_0|x)}{1 - P^\pi(\Theta_0|x)} = \frac{\pi_0}{1 - \pi_0} \times \text{BF}_{01}(x).$$

If $\Theta_0 = \{\theta_0\}$, then

$$\begin{aligned} \frac{\pi(\theta_0|x)}{1 - \pi(\theta_0|x)} &= \frac{\pi_0}{1 - \pi_0} \times \text{BF}_{01}(x) \\ \frac{1 - \pi(\theta_0|x)}{\pi(\theta_0|x)} &= \frac{1 - \pi_0}{\pi_0} \times \text{BF}_{01}^{-1}(x) \\ \frac{1}{\pi(\theta_0|x)} - 1 &= \frac{1 - \pi_0}{\pi_0} \times \text{BF}_{01}^{-1}(x) \\ \frac{1}{\pi(\theta_0|x)} &= 1 + \frac{1 - \pi_0}{\pi_0} \times \text{BF}_{01}^{-1}(x) \end{aligned}$$